theories/typing/uniq_bor.v
@@ -3,7 +3,7 @@ From iris.base_logic Require Import big_op.
 From lrust.lifetime Require Import borrow frac_borrow reborrow.
 From lrust.lang Require Import heap.
 From lrust.typing Require Export type.
-From lrust.typing Require Import lft_contexts type_context shr_bor perm typing programs.
+From lrust.typing Require Import lft_contexts type_context shr_bor programs.
 
 Section uniq_bor.
   Context `{typeG Σ}.
